HelloTypeSystem/Meta.lean
@@ -5,3 +5,4 @@ import «HelloTypeSystem».Meta.ReduceNatExpr
 import «HelloTypeSystem».Meta.Relation
 
 import «HelloTypeSystem».Meta.EvalML1
+import «HelloTypeSystem».Meta.TypingML1
