HelloTypeSystem/Meta/TypingML1.lean
@@ -1,0 +1,100 @@
+import HelloTypeSystem.ML1
+
+namespace HelloTypeSystem.ML1
+
+/-!
+# ML1に対する型付け
+
+## 型付けの例
+-/
+
+theorem «3 + 5 : int» : Derivable (⊢ 3 + 5 : Int) :=
+  ⟨.T_Plus .T_Int .T_Int⟩
+
+theorem «if 2 < 3 then 5 + 1 else 7 - 1 : int» : Derivable (⊢ .If (.LT 2 3) (5 + 1) (7 - 1) : Int) :=
+  ⟨.T_If
+    (.T_LT .T_Int .T_Int)
+    (.T_Plus .T_Int .T_Int)
+    (.T_Minus .T_Int .T_Int)
+  ⟩
+
+theorem «if 3 < 2 then 5 < 7 else 13 < 11 : bool» : Derivable (⊢ .If (.LT 3 2) (.LT 5 7) (.LT 13 11) : Bool) :=
+  ⟨.T_If
+    (.T_LT .T_Int .T_Int)
+    (.T_LT .T_Int .T_Int)
+    (.T_LT .T_Int .T_Int)
+  ⟩
+
+/-!
+## 型安全性
+-/
+
+set_option maxHeartbeats 0
+-- theorem type_safety : (dt : Derivation (⊢ e : τ)) → (de : Derivation (e ⇓ r)) → ∃ v : Value, r = .inr v ∧ ((τ = Int → ∃ i : Int, v = .Z i) ∨ (τ = Bool → ∃ b : Bool, v = .B b))
+--   | .T_Int,      .E_Int   (i := i)        => ⟨.Z i, rfl, .inl <| fun _ => ⟨i, rfl⟩⟩
+--   | .T_Bool,     .E_Bool  (b := b)        => ⟨.B b, rfl, .inr <| fun _ => ⟨b, rfl⟩⟩
+--   | .T_Plus _ _, .E_Plus  (i₃ := i) _ _ _ => ⟨.Z i, rfl, .inl <| fun _ => ⟨i, rfl⟩⟩
+--   -- | .T_Plus _ dt₂, .E_PlusIntBool (b₂ := b₂) _ de₂ =>
+--   --     have ⟨w, heq, h⟩ := type_safety dt₂ de₂
+--   --     -- have : ¬ Sum.inl Error.Plus = Sum.inr (Value.Z 0) := Sum.noConfusion
+--   --     have : False := ((Sum.inr.inj heq).symm ▸ h).elim
+--   --       (fun h => have ⟨_, h⟩ := h rfl; Value.noConfusion h)
+--   --       (fun h => h sorry)
+--   --       -- (fun ⟨0, h⟩ => Value.noConfusion h)
+--   --       -- (fun ⟨b, h⟩ => sorry)
+--   --     ⟨.Z 0, sorry, .inl ⟨0, rfl⟩⟩
+--   | .T_Minus _ _, _ => sorry
+--   | .T_Times _ _, _ => sorry
+--   | .T_LT _ _, _ => sorry
+--   | .T_If _ _ _, _ => sorry
+--   | _, _ => sorry
+
+theorem type_safety_ : (dt : Derivation (⊢ e : τ)) → (de : Derivation (e ⇓ r)) → ∃ v : Value, r = .inr v ∧ ((∃ i : Int, v = .Z i) ∨ (∃ b : Bool, v = .B b)) :=
+  fun dt de =>
+    match de with
+    | .E_Int   (i  := i)       => ⟨.Z i, rfl, .inl <| ⟨i, rfl⟩⟩
+    | .E_Bool  (b  := b)       => ⟨.B b, rfl, .inr <| ⟨b, rfl⟩⟩
+    | .E_Plus  (i₃ := i) _ _ _ => ⟨.Z i, rfl, .inl <| ⟨i, rfl⟩⟩
+    | .E_Minus (i₃ := i) _ _ _ => ⟨.Z i, rfl, .inl <| ⟨i, rfl⟩⟩
+    | .E_Times (i₃ := i) _ _ _ => ⟨.Z i, rfl, .inl <| ⟨i, rfl⟩⟩
+    | .E_LT    (b  := b) _ _ _ => ⟨.B b, rfl, .inr <| ⟨b, rfl⟩⟩
+    | .E_IfT   (v  := v) _ d   =>
+        ⟨v, rfl,
+          match dt with
+          | .T_If _ (.T_Int  (i := i)) _ => .inl <| match d with | .E_Int  => ⟨i, rfl⟩
+          | .T_If _ (.T_Bool (b := b)) _ => .inr <| match d with | .E_Bool => ⟨b, rfl⟩
+          | .T_If _ (.T_Plus dt₁ _)    _ => .inl <|
+              match d with
+              | .E_Plus (i₁ := i₁) (i₂ := i₂) de₁ _ (.B_Plus heq) =>
+                  have ⟨_, heq₁, h₁⟩ := type_safety_ dt₁ de₁
+                  h₁.elim
+                    (fun ⟨i, h⟩ => ⟨i₁ + i₂, heq ▸ rfl⟩)
+                    (fun ⟨b, h⟩ => (Sum.inr.inj heq₁).symm ▸ h |> Value.noConfusion)
+          | .T_If _ (.T_Minus dt₁ _) _ => .inl <|
+              match d with
+              | .E_Minus (i₁ := i₁) (i₂ := i₂) de₁ _ (.B_Minus heq) =>
+                  have ⟨_, heq₁, h₁⟩ := type_safety_ dt₁ de₁
+                  h₁.elim
+                    (fun ⟨i, h⟩ => ⟨i₁ - i₂, heq ▸ rfl⟩)
+                    (fun ⟨b, h⟩ => (Sum.inr.inj heq₁).symm ▸ h |> Value.noConfusion)
+          | .T_If _ (.T_Times dt₁ _) _ => .inl <|
+              match d with
+              | .E_Times (i₁ := i₁) (i₂ := i₂) de₁ _ (.B_Times heq) =>
+                  have ⟨_, heq₁, h₁⟩ := type_safety_ dt₁ de₁
+                  h₁.elim
+                    (fun ⟨i, h⟩ => ⟨i₁ * i₂, heq ▸ rfl⟩)
+                    (fun ⟨b, h⟩ => (Sum.inr.inj heq₁).symm ▸ h |> Value.noConfusion)
+          | .T_If _ (.T_LT _ _) _ => .inr <|
+              match d with
+              | .E_LT (b := true)  _ _ (.B_LTT _) => ⟨true,  rfl⟩
+              | .E_LT (b := false) _ _ (.B_LTF _) => ⟨false, rfl⟩
+          | .T_If _ (.T_If _ dt₂ dt₃) _ =>
+              match d with
+              | .E_IfT _ de₂ =>
+                  have ⟨_, heq, h⟩ := type_safety_ dt₂ de₂
+                  Sum.inr.inj heq ▸ h
+              | .E_IfF _ de₃ =>
+                  have ⟨_, heq, h⟩ := type_safety_ dt₃ de₃
+                  Sum.inr.inj heq ▸ h
+        ⟩
+    | _ => sorry
